Makefile
@@ -19,10 +19,12 @@ coq: Makefile.coq
 	mkdir -p ml
 	$(MAKE) -f Makefile.coq
 
-tmonad-gen: tmonad/insert_gen.v # more generated files go here
+tmonad-gen: tmonad/insert_gen.v tmonad/make_array_naive_gen.v
 
 tmonad/insert_gen.v: rkt/insert.rkt $(GEN_DEPS)
 	racket rkt/insert.rkt > tmonad/insert_gen.v
+tmonad/make_array_naive_gen.v: rkt/make_array_naive.rkt $(GEN_DEPS)
+	racket rkt/make_array_naive.rkt > tmonad/make_array_naive_gen.v
 
 Makefile.coq: tmonad-gen Makefile $(VS)
 	coq_makefile -R . Braun $(VS) -o Makefile.coq
